remove wf_res

theories/sim/invariant.v
@@ -35,7 +35,8 @@ Fixpoint active_SRO (stk: stack) : gset ptr_id :=
 
 Definition ptrmap_inv (r: resUR) (σ: state) : Prop :=
   ∀ (t: ptr_id) (k: tag_kind) h, r.1 !! t ≡ Some (to_tagKindR k, h) →
-  ∀ (l: loc) (s: scalar), h !! l ≡ Some (to_agree s) →
+  (t < σ.(snp))%nat ∧
+  (∀ (l: loc) (s: scalar), h !! l ≡ Some (to_agree s) →
   ∀ (stk: stack), σ.(sst) !! l = Some stk →
   ∀ pm opro, mkItem pm (Tagged t) opro ∈ stk →
   (* as long as the tag [t] is in the stack [stk],
@@ -46,7 +47,7 @@ Definition ptrmap_inv (r: resUR) (σ: state) : Prop :=
   match k with
   | tkUnique => ∃ stk' opro', stk = mkItem Unique (Tagged t) opro' :: stk'
   | tkPub => t ∈ active_SRO stk
-  end.
+  end).
 
 Definition cmap_inv (r: resUR) (σ: state) : Prop :=
   ∀ (c: call_id) (cs: callStateR), r.2 !! c ≡ Some cs →
@@ -63,7 +64,7 @@ Definition cmap_inv (r: resUR) (σ: state) : Prop :=
       (* then a c-protector must be in the stack of l *)
       ∃ stk pm, σ.(sst) !! l = Some stk ∧ mkItem pm (Tagged t) (Some c) ∈ stk
   (* if c is a public call id *)
-  | Cinr _ => True
+  | Cinr _ => (c < σ.(snc))%nat
   | _ => False
   end.
 
@@ -81,16 +82,10 @@ Definition srel (r: resUR) (σs σt: state) : Prop :=
   ∀ (l: loc) st, σt.(shp) !! l = Some st →
   (∃ ss, σs.(shp) !! l = Some ss ∧ arel r ss st) ∨ (∃ (t: ptr_id), priv_loc r l t).
 
-Record wf_res (r: resUR) (σ: state) : Prop := {
-  wf_res_call_id:
-    ∀ (c: call_id), c ∈ dom (gset call_id) r.2 → (c < σ.(snc))%nat;
-  wf_res_ptr_id :
-    ∀ (t: ptr_id), t ∈ dom (gset ptr_id) r.1 → (t < σ.(snp))%nat;
-}.
 
 Definition wsat (r: resUR) (σs σt: state) : Prop :=
   (* Wellformedness *)
-  Wf σs ∧ Wf σt ∧ wf_res r σt ∧ ✓ r ∧
+  Wf σs ∧ Wf σt ∧ ✓ r ∧
   (* Invariants *)
   ptrmap_inv r σt ∧ cmap_inv r σt ∧ srel r σs σt.
 
@@ -99,65 +94,6 @@ Definition wsat (r: resUR) (σs σt: state) : Prop :=
 Definition vrel (r: resUR) (v1 v2: value) := Forall2 (arel r) v1 v2.
 Definition vrel_expr (r: resUR) (e1 e2: expr) :=
   ∃ v1 v2, e1 = Val v1 ∧ e2 = Val v2 ∧ vrel r v1 v2.
-
-(* TODO: I hate these cmra operations *)
-Lemma ptrmap_inv_down_mono (r1 r2 : resUR) σ (VAL: ✓ r2) :
-  r1 ≼ r2 → ptrmap_inv r2 σ → ptrmap_inv r1 σ.
-Proof.
-  move => Le PI t k h Eqh l s Eqs stk Eqst pm opro IN.
-  have HL1: Some (to_tagKindR k, h) ≼ r2.1 !! t.
-  { rewrite -Eqh. by apply lookup_included, prod_included, Le. }
-  apply option_included in HL1 as [?|[? [[k' h'] [? [Eq1 INCL]]]]]; [done|].
-  simplify_eq.
-  have VL2: ✓ (k', h').
-  { apply (lookup_valid_Some _ t (k', h') (proj1 VAL)). by rewrite Eq1. }
-  assert (r2.1 !! t ≡ Some (to_tagKindR k, h') ∧ h ≼ h') as [Eq2 LE2].
-  { rewrite Eq1. move : INCL => [[/= EQ1 EQ2]|LE].
-    - by rewrite EQ1 EQ2.
-    - apply prod_included in LE as [Eq%tag_kind_incl_eq ?]; [|apply VL2].
-      simpl in Eq. by rewrite Eq. }
-  have EQL: h' !! l ≡ Some (to_agree s).
-  { move : LE2 => /lookup_included /(_ l). rewrite Eqs.
-    move => /option_included [//|[x [s' [? [EqL EqR]]]]]. simplify_eq.
-    rewrite EqL. move : EqR => [<-//|].
-    destruct (to_agree_uninj s') as [ss Eqss].
-    - apply (lookup_valid_Some h' l). apply VL2. by rewrite EqL.
-    - by rewrite -Eqss to_agree_included => ->. }
-  specialize (PI _ _ _ Eq2 _ _ EQL _ Eqst _ _ IN). naive_solver.
-Qed.
-
-Lemma cmap_inv_down_mono (r1 r2 : resUR) σ (VAL: ✓ r2) :
-  r1 ≼ r2 → cmap_inv r2 σ → cmap_inv r1 σ.
-Proof.
-  move => Le CI c cs Eqcs.
-  have HL1: Some cs ≼ r2.2 !! c.
-  { rewrite -Eqcs. by apply lookup_included, prod_included, Le. }
-  apply option_included in HL1 as [?|[cs1 [cs2 [? [Eq1 INCL]]]]]; [done|].
-  simplify_eq.
-  specialize (CI c cs2 (ltac: (by rewrite Eq1))).
-  have VL2: ✓ cs2.
-  { eapply (lookup_valid_Some r2.2 c). apply VAL. by rewrite Eq1. }
-  have VL1: ✓ cs1. { move : INCL => [-> //|]. by apply cmra_valid_included. }
-  destruct cs1 as [[T|]| |]; [|done..].
-  destruct INCL as [INCL|INCL]; last first.
-  { exfalso. apply (exclusive_included _ _ INCL VL2). }
-  destruct cs2 as [[T2|]| |]; [|done|by inversion INCL|done].
-  apply Cinl_inj, Excl_inj, leibniz_equiv_iff in INCL. subst T2.
-  destruct CI as [IN EQM]. split; [done|].
-  intros t INt k h Eqh l InD.
-  have HL1: Some (k, h) ≼ r2.1 !! t.
-  { rewrite -Eqh. by apply lookup_included, prod_included, Le. }
-  apply option_included in HL1 as [?|[? [[k' h'] [? [Eq2 INCL]]]]]; [done|].
-  simplify_eq.
-  have VL3: ✓ (k', h').
-  { apply (lookup_valid_Some _ t (k', h') (proj1 VAL)). by rewrite Eq2. }
-  assert (r2.1 !! t ≡ Some (k, h') ∧ h ≼ h') as [Eq3 LE2].
-  { rewrite Eq2. move : INCL => [[/= EQ1 EQ2]|LE].
-    - by rewrite EQ1 EQ2.
-    - apply prod_included in LE as [Eq%tag_kind_incl_eq ?]; [|apply VL3].
-      simpl in Eq. by rewrite Eq. }
-  apply (EQM _ INt k h' Eq3 l). eapply dom_included; eauto.
-Qed.
 
 Lemma arel_mono (r1 r2 : resUR) (VAL: ✓ r2) :
   r1 ≼ r2 → ∀ s1 s2, arel r1 s1 s2 → arel r2 s1 s2.
@@ -193,13 +129,6 @@ Proof.
   move => Le v1 v2 [? [? [? [? /(vrel_mono _ _ VAL Le) ?]]]]. do 2 eexists. eauto.
 Qed.
 
-Instance wf_res_proper : Proper ((≡) ==> (=) ==> iff) wf_res.
-Proof.
-  intros r1 r2 Eqr ???. subst.
-  split; intros [H1 H2]; (split; intros ? IN; [apply H1|apply H2]);
-    revert IN; apply dom_included; rewrite Eqr //.
-Qed.
-
 Instance ptrmap_inv_proper : Proper ((≡) ==> (=) ==> iff) ptrmap_inv.
 Proof.
   intros r1 r2 Eqr ? σ ?. subst. rewrite /ptrmap_inv. by setoid_rewrite Eqr.
@@ -231,3 +160,17 @@ Qed.
 
 Instance wsat_proper : Proper ((≡) ==> (=) ==> (=) ==> iff) wsat.
 Proof. solve_proper. Qed.
+
+Lemma cinv_lookup_in (r: resUR) (σ: state) c cs:
+  Wf σ → cmap_inv r σ → r.2 !! c ≡ Some cs → (c < σ.(snc))%nat.
+Proof.
+  intros WF CINV EQ. specialize (CINV c cs EQ).
+  destruct cs as [[]| |]; [|done..].
+  destruct CINV. by apply WF.
+Qed.
+
+Lemma cinv_lookup_in_eq (r: resUR) (σ: state) c cs:
+  Wf σ → cmap_inv r σ → r.2 !! c = Some cs → (c < σ.(snc))%nat.
+Proof.
+  intros WF CINV EQ. eapply cinv_lookup_in; eauto. by rewrite EQ.
+Qed.
